% ---------
%  Compile with "pdflatex hw0".
% --------
%!TEX TS-program = pdflatex
%!TEX encoding = UTF-8 Unicode

\documentclass[11pt]{article}
\usepackage{jeffe,handout,graphicx}
\usepackage[utf8]{inputenc}		% Allow some non-ASCII Unicode in source

%  Redefine suits
\usepackage{pifont}
\usepackage{algorithm}
\usepackage{algorithmic}
\usepackage{amsmath}
\documentclass{article}
\usepackage{amsmath}

\def\Spade{\text{\ding{171}}}
\def\Heart{\text{\textcolor{Red}{\ding{170}}}}
\def\Diamond{\text{\textcolor{Red}{\ding{169}}}}
\def\Club{\text{\ding{168}}}

\def\Cdot{\mathbin{\text{\normalfont \textbullet}}}
\def\Sym#1{\textbf{\texttt{\color{BrickRed}#1}}}


% =====================================================
%   Define common stuff for solution headers
% =====================================================
\Class{CS $450$}
\Semester{Spring $2019$}
\Authors{1}
%\Section{}

% =====================================================
\begin{document}

% ---------------------------------------------------------


% ---------------------------------------------------------
% Change authors again
\AuthorOne{Ray Ying}{xinruiy2@illinois.edu}


\HomeworkHeader{$9$}{$1$}

\begin{quote}

\end{quote}
\hrule


\begin{solution}
\item  
    $f(x) = h(x)(x - x^*)^{m}$\\
    $f'(x) = h'(x)(x - x^*)^{m} + m\cdot h(x)(x - x^*)^{m-1}$\\
    $f''(x) = h''(x)(x-x^*)^m + 2m\cdot h'(x)(x-x^*)^{m-1} + m(m-1)h(x)(x-x^*)^{m-2}$
        \begin{enumerate}
            \item $g(x) = x - \frac{h(x)(x - x^*)^{m}}{m \cdot (x - x^*)^{m-1}h(x) + h'(x)(x - x^*)^{m}} = x - \frac{h(x)(x - x^*)}{m \cdot h(x) + h'(x)(x - x^*)}$

            \item $g'(x) = 1 - \frac{(m \cdot h(x) + h'(x)(x - x^*)) \cdot (h(x) + h'(x)(x-x^*))- h(x)(x-x^*)(m \cdot h'(x) + h''(x)(x-x^*) + h'(x))}{(m \cdot h(x) + h'(x)(x - x^*))^2} \\
            = 1 - \frac{(m \cdot h(x) + h'(x)(x - x^*)) \cdot (h(x) + h'(x)(x-x^*))- h(x)(x-x^*)(m \cdot h'(x) + h''(x)(x-x^*) + h'(x))}{(m \cdot h(x) + h'(x)(x - x^*))^2}$\\
            = $\frac{(m \cdot h(x) + h'(x)(x - x^*))^2 - (m \cdot h(x) + h'(x)(x - x^*)) \cdot (h(x) + h'(x)(x-x^*))+ h(x)(x-x^*)(m \cdot h'(x) + h''(x)(x-x^*) + h'(x))}{(m \cdot h(x) + h'(x)(x - x^*))^2}$\\
            
            $g'(x^*) = \frac{(m\cdot h(x^*))^2 - m\cdot h(x^*)^2}{(m\cdot h(x^*))^2} = 1 - \frac{1}{m}$
            \\
            Because $m \neq 0$, $g'(x^*) \neq 0$ for all $x^*$. Therefore, it's linearity convergence. 
            
            \item Having $g(x) = x - k\cdot f(x)/f'(x)$, $g(x) = x - \frac{k\cdot h(x)(x - x^*)}{ m \cdot h(x) + h'(x)(x - x^*)} $\\
            
            $g'(x) = 1 - \frac{k \cdot (m \cdot h(x) + h'(x)(x - x^*)) \cdot (h(x) + h'(x)(x-x^*))- k \cdot h(x)(x-x^*)(m \cdot h'(x) + h''(x)(x-x^*) + h'(x))}{(m \cdot h(x) + h'(x)(x - x^*))^2}$\\
            
            When $g'(x^*) = 0$, it has quadratic convergence.\\
            $1 =  \frac{k \cdot m \cdot h(x)^2}{m^2h(x)^2} \implies k = m$\\
            
            
            
        \end{enumerate}
    
\end{solution}
References: \\ 

\end{document}
