% ---------
%  Compile with "pdflatex hw0".
% --------
%!TEX TS-program = pdflatex
%!TEX encoding = UTF-8 Unicode

\documentclass[11pt]{article}
\usepackage{jeffe,handout,graphicx}
\usepackage[utf8]{inputenc}		% Allow some non-ASCII Unicode in source

%  Redefine suits
\usepackage{pifont}
\usepackage{algorithm}
\usepackage{algorithmic}
\usepackage{amsmath}

\def\Spade{\text{\ding{171}}}
\def\Heart{\text{\textcolor{Red}{\ding{170}}}}
\def\Diamond{\text{\textcolor{Red}{\ding{169}}}}
\def\Club{\text{\ding{168}}}

\def\Cdot{\mathbin{\text{\normalfont \textbullet}}}
\def\Sym#1{\textbf{\texttt{\color{BrickRed}#1}}}


% =====================================================
%   Define common stuff for solution headers
% =====================================================
\Class{CS $450$}
\Semester{Spring $2019$}
\Authors{1}
%\Section{}

% =====================================================
\begin{document}

% ---------------------------------------------------------


% ---------------------------------------------------------
% Change authors again
\AuthorOne{Ray Ying}{xinruiy2@illinois.edu}


\HomeworkHeader{$3$}{$1$}

\begin{quote}

\end{quote}
\hrule


\begin{solution}
\item
\begin{enumerate}
    \item 
    Based on the two equation given: $\hat{A} = A + \delta A $ and $\hat{x} = x - \delta x$. \\
    $\hat{A}\hat{x} = (A  + \delta A)(x -  \delta x) = Ax - A\delta x + x\delta A - \delta A \delta x = Ax - A\delta x + x\delta A = b $. \\
    We have that $Ax = b$, delete on both side of above equation:\\
    $ A\delta x = \delta A x \implies \delta x = A^{-1}\delta A x \implies \abs{\delta x} = \abs{A^{-1}\delta A x} \implies \norm {\abs{\delta x}} = \norm {\abs{A^{-1}\delta A x}} \implies \norm {\abs{\delta x}} \leq \norm{\abs{A^{-1}}} \cdot  \norm{\abs{\delta A}} \cdot \norm{\abs{x}}. $\\
    Based on the definition of $\epsilon \geq$ max$_{i,j} \abs{\delta a_{i,j}/ a_{i,j}}$, it guarantees that $\norm {\abs {\delta A}} \leq \epsilon \norm{\abs{A}} \implies \norm {\delta A} \leq \epsilon \norm{A}$.
    Therefore, the inequality we derived before can be transform into the inequality we want to prove:\\
    $\norm {\abs{\delta x}} \leq \norm{\abs{A^{-1}}} \cdot  \norm{\abs{\delta A}} \cdot \norm{\abs{x}} \implies \frac{\norm {\abs{\delta x}}}{\norm{x}}\leq \norm{\abs{A^{-1}}} \cdot  \norm{\abs{\delta A}} \implies \frac{\norm {\abs{\delta x}}}{\norm{x}}\leq \epsilon \norm{\abs{A^{-1}}} \cdot  \norm{\abs{A}} \implies \frac{\norm {\abs{\delta x}}}{\norm{x}}\leq \epsilon \norm{\abs{A^{-1}} \cdot \abs{A}} \implies \frac{\norm {x - \hat{x}}}{\norm{x}}\leq \epsilon \norm{\abs{A^{-1}} \cdot \abs{A}}$.\\
    Hence, proved.
    
    
    \item Proof:
    \newline
        $K_{CR}(DA) = \norm{ \abs{(DA)^{-1}} \cdot \abs{(DA)} } = \norm { \abs{A^{-1}D^{-1}} \cdot \abs{DA}} = \norm {\abs{A^{-1}D^{^-1}DA}} = \norm {\abs {A^{-1}A}} = \norm {\abs {A^{-1}} \abs A } = K_{CR}(A)$.\\
        Hence, proved.
        
    \end{enumerate}
    (The norm above is $1$-norm)
\end{solution}
\end{document}
