% ---------
%  Compile with "pdflatex hw0".
% --------
%!TEX TS-program = pdflatex
%!TEX encoding = UTF-8 Unicode

\documentclass[11pt]{article}
\usepackage{jeffe,handout,graphicx}
\usepackage[utf8]{inputenc}		% Allow some non-ASCII Unicode in source

%  Redefine suits
\usepackage{pifont}
\usepackage{algorithm}
\usepackage{algorithmic}
\usepackage{amsmath}
\documentclass{article}
\usepackage{amsmath}

\def\Spade{\text{\ding{171}}}
\def\Heart{\text{\textcolor{Red}{\ding{170}}}}
\def\Diamond{\text{\textcolor{Red}{\ding{169}}}}
\def\Club{\text{\ding{168}}}

\def\Cdot{\mathbin{\text{\normalfont \textbullet}}}
\def\Sym#1{\textbf{\texttt{\color{BrickRed}#1}}}


% =====================================================
%   Define common stuff for solution headers
% =====================================================
\Class{CS $450$}
\Semester{Spring $2019$}
\Authors{1}
%\Section{}

% =====================================================
\begin{document}

% ---------------------------------------------------------


% ---------------------------------------------------------
% Change authors again
\AuthorOne{Ray Ying}{xinruiy2@illinois.edu}


\HomeworkHeader{$10$}{$1$}

\begin{quote}

\end{quote}

\hrule

\begin{solution}
\item 

\begin{enumerate}
    \item $\Phi(x) = \frac{1}{2}((x+1)^2 + (\lambda x^2 + x - 1)^2)$\\
    $\Phi'(x) = 2 \lambda^2 x^3 + 3 \lambda x^2 - 2 \lambda x + 2x$\\
    $\Phi''(x) = 6 \lambda^2 x^2 + 6\lambda x - 2\lambda + 2$\\
    
    If $\lambda < 1$ and $x = 0$, $\Phi'(x) = 0$ and $\Phi''(x) = 2 - 2\lambda \geq 0$ $\implies$ it has local minimum at $x = 0$.\\
    
    If $\lambda < \frac{7}{16}$, there are two complex roots and only one real root at $x = 0$.\\
    
    \item  $x_{k+1} = x_k + s_k$\\
    $J_{xk}s_k \cong -F(x_k) \implies s_k =- (J^T \cdot J)^{-1}\cdot J^T \cdot F(x_k)$\\
    $J = [1 ,2 \lambda x_k + 1] \implies J^T\cdot J = 1 + (2 \lambda x_k + 1)^2$\\
    $g(x) = x_k - \frac{1}{1 + (2 \lambda x_k + 1)^2}\cdot J^T \cdot F(x_k) = x_k - \frac{1 + x + (2 \lambda x_k + 1)(\lambda x^2 + x - 1)}{1 + (2 \lambda x_k + 1)^2}$\\
    $g'(x) = 1 - (\frac{\lambda}{2\lambda^2x^2+2\lambda x+1} + \frac{-4 \lambda^2 x + 2\lambda x- 4\lambda + 1}{2(2\lambda^2 x^2+2\lambda x+ 1)^2} + \frac{1}{2})$\\
    $g'(x = 0) = 1 - (\lambda + \frac{-4\lambda + 1}{2} + \frac{1}{2}) = 1 - \lambda + 2\lambda - 1 = \lambda \implies |g'(x = 0)| = |\lambda| > 1 $ \\
    
    
    \item Using Levenberg-Marquardt method, 
    $s_k =- (J^T \cdot J + \lambda I)^{-1}\cdot J^T \cdot F(x_k)$,\\
    $g(x) = x_k - (J^T \cdot J + |\lambda| I)^{-1}\cdot J^T \cdot F(x_k) = x_k - \frac{1 + x + (2 \lambda x_k + 1)(\lambda x^2 + x - 1)}{1 + (2 \lambda x_k + 1)^2 + |\lambda|}$\\
    $g'(x) = 1 - \frac{2(4\lambda^4x^4 + 8 \lambda^3x^3 + 4a^3x^2+3a^2x^2|\lambda| + 8\lambda^2 x^2+ 3\lambda x|\lambda| - \lambda|\lambda| + |\lambda| + 6\lambda x - 2\lambda +2 )}{(4\lambda^2x^2 + |\lambda| + 4\lambda x + 2)^2}$\\
    $g'(x = 0) = 1 - \frac{2(-|\lambda|\lambda + |\lambda| - \lambda + 2)}{(|\lambda| + 2)^2}$\\
    
    Given $\lambda < \frac{7}{16}$, we divided into $\lambda < 0$ and $\frac{7}{16} > \lambda \geq 0$.\\
    
    $\lambda < 0$, $|\lambda| = -\lambda$. $g'(x = 0) = 1 - \frac{2(\lambda^2 - 2\lambda + 2)}{(2 - \lambda)^2} = 1 - \frac{(2-\lambda)^2+\lambda^2}{(2-\lambda^2)} = \frac{\lambda^2}{(2-\lambda)^2}$. Since $\lambda < 0$, $(2-\lambda)^2 > \lambda^2 \implies \frac{\lambda^2}{(2-\lambda)^2} < 1$. Also, both $\lambda^2$ and $(2-\lambda)^2$ are greater than $0$, $\frac{\lambda^2}{(2-\lambda)^2} > 0$. Thus, $|g'(x = 0)| < 1$ $\forall { \lambda < 0}$\\
    
    $\frac{7}{16} > \lambda \geq 0$, $|\lambda| = \lambda$. $g'(x = 0) = 1 - \frac{2(\lambda^2 + 2)}{(\lambda + 2)^2}$. Since both $2(\lambda^2 + 2)$ and $(\lambda + 2)^2$ are greater than $0$, $\frac{2(\lambda^2 + 2)}{(\lambda + 2)^2} > 0 \implies g'(x = 0) < 1$.\\
    $2(\lambda^2 + 2) - (\lambda + 2)^2  = \lambda^2 - 4\lambda < 0 \implies \frac{2(\lambda^2 + 2)}{(\lambda + 2)^2} < 1 \implies g'(x = 0) > 0$\\
    Thus, $|g'(x = 0)| < 1$ $\forall { \frac{7}{16} > \lambda \geq 0}$\\
    
    Therefore, when $\lambda < \frac{7}{16}$, $|g'(x=0)| < 1$
    
    
\end{enumerate}

\end{solution}
References: \\ 

\end{document}
